working on stack introduction

src/Dmajortodflatmajor.v
@@ -25,12 +25,8 @@ Section PRESERVATION.
 Variable prog: Dmajor.program.
 Let ge := Genv.globalenv prog.
 
-(* given a continuation, memory, injection, current stack size and current stack pointer *)
-(* need that: *)
-(* 1. current sp not in injection *)
-(* 2. current stack frame is freeable *)
-(* 1 and 2 hold for stack frames in continuation *)
 
+(* Here we have a sufficient condition which we'll prove holds on all stack frames *)
 Definition stack_frame_wf (b : block) (stacksize : Z) (mi : meminj) (m : mem) : Prop :=
    Mem.range_perm m b 0 stacksize Cur Freeable /\ forall b' delta, mi b' <> Some (b,delta).
 
@@ -51,60 +47,80 @@ Proof.
   specialize (H1 b' delta). congruence.
 Qed.
 
+(* Here we have properties about the memory injection *)
+
+(* This says that our injection maps every old block to something new *)
 Definition total_inj (mi : meminj) (m : mem) : Prop :=
   forall c b ofs v,
     Mem.load c m b ofs = Some v ->
     exists b',
       mi b = Some (b',0).
 
+(* local variables follow our injection *)
 Definition env_inj (mi : meminj) (e e' : env) : Prop :=
   forall id v,
     e ! id = Some v ->
     exists v',
       e' ! id = Some v' /\ Val.inject mi v v'.
 
-(* HERE *)
-(* TODO do these next *)
-(* We need fact that all globals inject to same *)
+(* globals aren't moved around *)
+Definition globals_inj_same (mi : meminj) : Prop :=
+  forall i b,
+    Genv.find_symbol ge i = Some b ->
+    mi b = Some (b,0).
 
-(* we need a fact about the injection *)
-(* that we'll never grab something not in the injection *)
+(* evaluating expressions translates *)
 Lemma eval_expr_mem_inj :
-  forall ge e m exp v,
+  forall e m exp v,
     Dmajor.eval_expr ge e m exp v ->
     forall m' mi e' sp,
       Mem.mem_inj mi m m' ->
       total_inj mi m ->
       env_inj mi e e' ->
+      globals_inj_same mi ->
       exists v',
         eval_expr ge e' m' sp exp v' /\ Val.inject mi v v'.
 Proof.
-  (* induction 1; intros; *)
-  (*   try (app H2 (e ! id)). *)
-  (* eexists; split; try econstructor; eauto. *)
-  (* eexists; split; try econstructor; eauto. *)
-  (* unfold Dmajor.eval_constant in *. *)
+  induction 1; intros.
+  * copy H; try eapply H2 in H;
+      repeat break_exists; repeat break_and;
+        try solve [eexists; split; try econstructor; eauto].
+  * eexists; split.
+    econstructor; eauto.
+    unfold Dmajor.eval_constant in *.
+    break_match_hyp; try congruence; find_inversion.
+    econstructor; eauto.
+    break_match; econstructor; eauto.
+    ring.
+  * edestruct IHeval_expr1; eauto.
+    edestruct IHeval_expr2; eauto.
+    break_and.
+    eexists; eauto. split.
+    econstructor; eauto.
+    eapply Val.add_inject; eauto.
+  *
+    destruct vaddr; simpl in H0; try congruence.
+    destruct (mi b) eqn:?.
+    destruct p.
+    app Mem.load_inj Mem.load.
+    
+    edestruct IHeval_expr; eauto.
+    break_and.
+    inv H8.
 
-  (* break_match_hyp; inv H; try econstructor; eauto. *)
-  
-  (*   try solve [eexists; split; econstructor; eauto]. *)
-  (* * app H2 (e ! id). *)
-  (* eexists. split. econstructor; eauto. *)
-  
-  (*   try solve [eexists; split; econstructor; eauto]. *)
-  
-  (* destruct vaddr; simpl in *; try congruence. *)
-  (* copy H1. *)
-  (* app H2 Mem.load. *)
-  
-  (* eapply Mem.load_inj in H1; eauto. *)
-  (* break_exists. break_and. *)
-  (* rewrite Zplus_0_r in H1. *)
-  
-  (* econstructor; try eapply IHeval_expr; eauto. *)
-  (* simpl.  *)
-  (* app Mem.load_inj Mem.mem_inj. *)
-  (* SearchAbout Mem.mem_inj. *)
+    eexists; split.
+    econstructor; eauto.
+    simpl. 
+    erewrite <- H0.
+    f_equal. 
+    congruence.
+
+    admit. (* whatever *)
+
+    eauto.
+    edestruct IHeval_expr; eauto.
+    break_and. inv H6. congruence.
+
 Admitted.
 
 Inductive match_cont : Dmajor.cont -> Dflatmajor.cont -> Prop :=
@@ -116,33 +132,71 @@ Inductive match_cont : Dmajor.cont -> Dflatmajor.cont -> Prop :=
 | match_block : forall k k',
     match_cont k k' ->
     match_cont (Dmajor.Kblock k) (Dflatmajor.Kblock k')
-| match_call : forall oid f e sp k k',
+| match_call : forall oid f e e' sp k k' mi,
     match_cont k k' ->
-    (* TODO: need similar but not same envs *)
-    match_cont (Dmajor.Kcall oid f e k) (Dflatmajor.Kcall oid f sp e k').
+    env_inj mi e e' ->
+    match_cont (Dmajor.Kcall oid f e k) (Dflatmajor.Kcall oid f sp e' k').
 
 
 Inductive match_states : Dmajor.state -> Dflatmajor.state -> Prop :=
-| match_state : forall f s k k' b e m m' z mi,
+| match_state : forall f s k k' b e e' m m' z mi,
     Mem.mem_inj mi m m' ->
     stack_frame_wf b (fn_stackspace f) mi m' ->
     match_cont k k' ->
+    total_inj mi m ->
+    env_inj mi e e' ->
+    globals_inj_same mi ->
+    Mem.meminj_no_overlap mi m ->
     match_states
       (Dmajor.State f s k e m)
-      (Dflatmajor.State f s k' (Vptr b Int.zero) e m' z)
+      (Dflatmajor.State f s k' (Vptr b Int.zero) e' m' z)
 | match_callstate : forall f args k k' m m' z mi,
     Mem.mem_inj mi m m' ->
     match_cont k k' ->
+    total_inj mi m ->
+    globals_inj_same mi ->
+    Mem.meminj_no_overlap mi m ->
     match_states
       (Dmajor.Callstate f args k m)
       (Dflatmajor.Callstate f args k' m' z)
 | match_returnstate : forall v k k' m m' z mi,
     Mem.mem_inj mi m m' ->
     match_cont k k' ->
+    total_inj mi m ->
+    globals_inj_same mi ->
+    Mem.meminj_no_overlap mi m ->
     match_states
       (Dmajor.Returnstate v k m)
       (Dflatmajor.Returnstate v k' m' z).
 
+Lemma is_call_cont_transf :
+  forall k k',
+    match_cont k k' ->
+    Dmajor.is_call_cont k ->
+    is_call_cont k'.
+Proof.
+  induction k; intros;
+    inv H; eauto.
+Qed.
+
+Lemma env_inj_set :
+  forall mi e e',
+    env_inj mi e e' ->
+    forall id v x,
+      Val.inject mi v x ->
+      env_inj mi (PTree.set id v e) (PTree.set id x e').
+Proof.
+Admitted.
+
+Lemma total_inj_store_mapped :
+  forall mi m,
+    total_inj mi m ->
+    forall c b ofs v m',
+      Mem.store c m b ofs v  = Some m' ->
+      exists b' delta,
+        mi b = Some (b',delta).
+Proof.
+Admitted.
 
 Lemma single_step_correct:
   forall S1 t S2, Dmajor.step ge S1 t S2 ->
@@ -151,10 +205,27 @@ Lemma single_step_correct:
 Proof.
   intros.
   
-  inv H0; inv H; try inv H3;
-    
-    try solve [eexists; split; try eapply plus_one; econstructor; eauto].
-  eexists; split; try eapply plus_one; econstructor; eauto.
+  inv H0; inv H;
+  try solve [inv H3;
+             eexists; split; try eapply plus_one; econstructor; eauto].
+  * app free_stack_frame stack_frame_wf; eauto.
+    eexists; split; try eapply plus_one; econstructor; eauto.
+    eapply is_call_cont_transf; eauto.
+  * app eval_expr_mem_inj Dmajor.eval_expr.
+    eexists; split; try eapply plus_one; econstructor; eauto.
+    eapply env_inj_set; eauto.
+  * app eval_expr_mem_inj (Dmajor.eval_expr ge e m addr vaddr).
+    app eval_expr_mem_inj (Dmajor.eval_expr ge e m a v).
+    destruct vaddr; simpl in *; try congruence.
+    app total_inj_store_mapped total_inj.
+    app Mem.store_mapped_inj Mem.mem_inj.
+    inv H10.    
+    eexists; split; try eapply plus_one; econstructor; eauto.
+    simpl. rewrite <- H1.
+    f_equal; try congruence.
+    admit. (* grumble ints *)
+
+
   
 Admitted.
 
